wip!

Lp2lc/Active/DTLC/Def.lean
@@ -24,7 +24,7 @@ inductive Typ : Type (u + 1) where
 | depFn (tIn : Typ) (tOut : (arg : I) -> Typ) : Typ
 
 inductive Trm : Type (u + 1) where
-| var (symbol : I) (tAnnotation : Typ) : Trm
+| var (symbol : I) {tAnnotation : Typ} : Trm
 | val (v : Val) : Trm
 | depApply (fn : Trm) (arg : Trm) : Trm
 
@@ -35,66 +35,24 @@ end
 
 end Syntax
 
-abbrev TrmClosed := {I : Sort 1} -> Trm I
+abbrev TrmClosed := {I : Sort u} -> Trm I
 
-abbrev TypClosed := {I : Sort 1} -> Typ I
+abbrev TypClosed := {I : Sort u} -> Typ I
 
-abbrev ByteCodeTrm := Trm ByteCode
+structure RuntimeCarrier where
+  self: ByteCode
 
-abbrev ByteCodeVal := Val ByteCode
-
-section Semantics
-
-@[simp]
-private def evalBytecode (fuel : Nat) (trm : ByteCodeTrm) : Option ByteCodeVal :=
-  match fuel with
-  | 0 => none
-  | fuel + 1 =>
-      match trm with
-      | Trm.var symbol _ => some (Val.primitive symbol)
-      | Trm.val (Val.primitive repr) => some (Val.primitive repr)
-      | Trm.val (Val.depFn body) => some (Val.depFn body)
-      | Trm.depApply fn arg =>
-          match evalBytecode fuel fn, evalBytecode fuel arg with
-          | some (Val.depFn body), some (Val.primitive argByte) =>
-              evalBytecode fuel (body argByte)
-          | _, _ => none
-
-@[simp]
-private def typingBytecode (fuel : Nat) (trm : ByteCodeTrm) (typ : Typ ByteCode) : Prop :=
-  match fuel with
-  | 0 => False
-  | fuel + 1 =>
-      match trm with
-      | Trm.var _ tAnnotation => tAnnotation = typ
-      | Trm.val (Val.primitive _) => typ = Typ.primitive
-      | Trm.val (Val.depFn body) =>
-          match typ with
-          | Typ.primitive => False
-          | Typ.depFn tIn tOut =>
-              ∀ arg : ByteCode,
-                typingBytecode fuel (Trm.val (Val.primitive arg)) tIn ->
-                typingBytecode fuel (body arg) (tOut arg)
-      | Trm.depApply fn arg =>
-          ∃ tIn tOut argByte,
-            typingBytecode fuel fn (Typ.depFn tIn tOut) ∧
-            typingBytecode fuel arg tIn ∧
-            evalBytecode fuel arg = some (Val.primitive argByte) ∧
-            typ = tOut argByte
+abbrev RuntimeVal := Val RuntimeCarrier
 
 namespace TrmClosed
 
 @[simp]
-def eval (trm : TrmClosed) (fuel : Nat) : Option ByteCodeVal :=
-  evalBytecode fuel (trm (I := ByteCode))
+def eval (trm : TrmClosed) (fuel : Nat) : Option RuntimeVal := sorry
 
-@[simp]
-def typing (trm : TrmClosed) (fuel : Nat) (typ : TypClosed) : Prop :=
-  typingBytecode fuel (trm (I := ByteCode)) (typ (I := ByteCode))
+-- @[simp]
+-- def typing (trm : TrmClosed) (fuel : Nat) (typ : TypClosed) : Prop := sorry
 
 end TrmClosed
-
-end Semantics
 
 end DTLC
 
